Spacetalk/Step.lean
@@ -1,4 +1,5 @@
 import Spacetalk.Stream
+import Spacetalk.HList
 
 -- Source Lang
 namespace Step
@@ -16,11 +17,17 @@ inductive Ty
   | stream : Prim → Ty
   deriving DecidableEq
 
+@[simp]
+def Ty.prim : Ty → Prim
+  | stream p => p
+
 infixr:25 " → " => Ty.fn
 
 @[reducible]
 def Ty.denote : Ty → Type
   | stream p => Stream' p.denote
+
+abbrev TysInput (tys : List Ty) := HList Ty.denote tys
 
 inductive BinaryOp : Prim → Prim → Prim → Type
   | add : {w : Nat} → BinaryOp (.bitVec w) (.bitVec w) (.bitVec w)
@@ -30,11 +37,11 @@ inductive UnaryOp : Prim → Prim → Type
   | addConst : {w : Nat} → BitVec w → UnaryOp (.bitVec w) (.bitVec w)
   | mulConst : {w : Nat} → BitVec w → UnaryOp (.bitVec w) (.bitVec w)
 
-inductive Prog : Ty → Type
-  | const : (α : Ty) → α.denote → Prog α
-  | zip : BinaryOp α β γ → Prog (.stream α) → Prog (.stream β) → Prog (.stream γ)
-  | map : UnaryOp α β → Prog (.stream α) → Prog (.stream β)
-  | reduce : BinaryOp α β α → Nat → α.denote → Prog (.stream β) → Prog (.stream α)
+inductive Prog : List Ty → Ty → Type
+  | const : (α : Ty) → Prog [α] α
+  | zip : BinaryOp α β γ → Prog aInp (.stream α) → Prog bInp (.stream β) → Prog (aInp ++ bInp) (.stream γ)
+  | map : UnaryOp α β → Prog inp (.stream α) → Prog inp (.stream β)
+  | reduce : BinaryOp α β α → Nat → α.denote → Prog inp (.stream β) → Prog inp (.stream α)
 
 ------------------ Semantics ------------------
 def BinaryOp.denote : BinaryOp α β γ → α.denote → β.denote → γ.denote
@@ -45,15 +52,9 @@ def UnaryOp.denote : UnaryOp α β → α.denote → β.denote
   | UnaryOp.addConst c => BitVec.add c
   | UnaryOp.mulConst c => BitVec.mul c
 
-def Prog.denote {α : Ty} : Prog α → α.denote
-  | .const _ a => a
-  | .zip op as bs => Stream'.zip op.denote as.denote bs.denote
-  | .map op as => Stream'.map op.denote as.denote
-  | .reduce op n init bs => Stream'.reduce op.denote n init bs.denote
-
-def Prog.p : Prog α → List Nat
-  | .const _ _ => [1]
-  | .zip _ as bs => as.p ++ bs.p
-  | .map _ as => as.p
-  | .reduce _ _ _ bs => bs.p
+def Prog.denote {inputs : List Ty} {α : Ty} : Prog inputs α → (TysInput inputs → TysInput [α])
+  | .const _ => λ ([a]ₕ) ↦ [a]ₕ
+  | .zip op as bs => λ inp ↦ let (aInp, bInp) := inp.split; [Stream'.zip op.denote (as.denote aInp).head (bs.denote bInp).head]ₕ
+  | .map op as => λ inp ↦ [Stream'.map op.denote (as.denote inp).head]ₕ
+  | .reduce op n init bs => λ inp ↦ [Stream'.reduce op.denote n init (bs.denote inp).head]ₕ
 end Step
